SciLean/Tactic/MathlibCompiledTactics.lean
@@ -1,3 +1,5 @@
 import Mathlib.Tactic.FunProp
 import Mathlib.Tactic.FunTrans.Elab
 import Mathlib.Tactic.FunTrans.Attr
+import SciLean.Tactic.LSimp.Elab
+import SciLean.Tactic.LSimp.Main
