test/lsimp_basic_tests.lean
@@ -1,100 +1,177 @@
 import SciLean.Tactic.LSimp.Elab
 import SciLean.Util.RewriteBy
 import SciLean.Core
-
-example (n : Nat) :
-  n
-  =
-  n := by (conv => lhs; lsimp)
-
-example (n : Nat) :
-  (let a := 1; a + n)
-  =
-  (1 + n) := by (conv => lhs; lsimp)
-
-example (n : Nat) :
-  (0 + n)
-  =
-  n := by (conv => lhs; lsimp)
-
-example (n : Nat) :
-  (0 + 1 * n)
-  =
-  n := by (conv => lhs; lsimp)
-
-example (n : Nat) :
-  (let a := (0 + 1 * n); a)
-  =
-  n := by (conv => lhs; lsimp)
-
-example (n : Nat) :
-    (let a :=
-       let c := 0 + n
-       let d := c + 0 + 3
-       c + d + 1 * n + 2
-     let b := a + 5
-     a + b)
-    =
-    n + (n + 3) + n + 2 + (n + (n + 3) + n + 2 + 5) := by
-  (conv => lhs; lsimp)
-
-example (n : Nat) (i : Fin n) :
-    (let j := 2*i.1
-     let hj : j < 2*n := by omega
-     let j : Fin (2*n) := ⟨j, hj⟩
-     let k :=
-       let a := j + j
-       a + j
-     j + k)
-    =
-    let j := 2*i.1
-    let hj : j < 2*n := by omega
-    let j : Fin (2*n) := ⟨j, hj⟩
-    (j + (j + j + j)) := by
-  (conv => lhs; lsimp)
-
--- tests under lambda binder
-
-example :
-  (fun n : Nat => n)
-  =
-  (fun n : Nat => n) := by (conv => lhs; lsimp)
-
-example :
-  (fun n => let a := 1; a + n)
-  =
-  (fun n => 1 + n) := by (conv => lhs; lsimp)
+import SciLean.Tactic.MathlibCompiledTactics
+import SciLean.Util.Profile
 
 
-example :
-  (fun n => let a := (0 + 1 * n); a)
-  =
-  (fun n => n) := by (conv => lhs; lsimp)
+-- example (n : Nat) :
+--   n
+--   =
+--   n := by (conv => lhs; lsimp)
+
+-- example (n : Nat) :
+--   (let a := 1; a + n)
+--   =
+--   (1 + n) := by (conv => lhs; lsimp)
+
+-- example (n : Nat) :
+--   (0 + n)
+--   =
+--   n := by (conv => lhs; lsimp)
+
+-- example (n : Nat) :
+--   (0 + 1 * n)
+--   =
+--   n := by (conv => lhs; lsimp)
+
+-- example (n : Nat) :
+--   (let a := (0 + 1 * n); a)
+--   =
+--   n := by (conv => lhs; lsimp)
+
+-- example (n : Nat) :
+--     (let a :=
+--        let c := 0 + n
+--        let d := c + 0 + 3
+--        c + d + 1 * n + 2
+--      let b := a + 5
+--      a + b)
+--     =
+--     n + (n + 3) + n + 2 + (n + (n + 3) + n + 2 + 5) := by
+--   (conv => lhs; lsimp)
+
+-- example (n : Nat) (i : Fin n) :
+--     (let j := 2*i.1
+--      let hj : j < 2*n := by omega
+--      let j : Fin (2*n) := ⟨j, hj⟩
+--      let k :=
+--        let a := j + j
+--        a + j
+--      j + k)
+--     =
+--     let j := 2*i.1
+--     let hj : j < 2*n := by omega
+--     let j : Fin (2*n) := ⟨j, hj⟩
+--     (j + (j + j + j)) := by
+--   (conv => lhs; lsimp)
+
+-- -- tests under lambda binder
+
+-- example :
+--   (fun n : Nat => n)
+--   =
+--   (fun n : Nat => n) := by (conv => lhs; lsimp)
+
+-- example :
+--   (fun n => let a := 1; a + n)
+--   =
+--   (fun n => 1 + n) := by (conv => lhs; lsimp)
 
 
-example :
-    (fun n : Nat=>
-     let c := n
-     let a := c + 1 * n
-     a)
-    =
-    (fun n => n + n) := by
-  (conv => lhs; lsimp)
+-- example :
+--   (fun n => let a := (0 + 1 * n * 1 * 2); a)
+--   =
+--   (fun n => n * 2) := by (conv => lhs; lsimp)
 
 
-example :
-    (fun (n : Nat) (i : Fin n) =>
-     let j := 2*i.1
-     let hj : j < 2*n := by omega
-     let j : Fin (2*n) := ⟨j, hj⟩
-     let k :=
-       let a := j + j
-       a + j
-     j + k)
-    =
-    fun (n : Nat) (i : Fin n) =>
-    let j := 2*i.1
-    let hj : j < 2*n := by omega
-    let j : Fin (2*n) := ⟨j, hj⟩
-    (j + (j + j + j)) := by
-  (conv => lhs; lsimp)
+-- example :
+--     (fun n : Nat=>
+--      let c := n
+--      let a := c + 1 * n
+--      a)
+--     =
+--     (fun n => n + n) := by
+--   (conv => lhs; lsimp)
+
+
+-- example :
+--     (fun (n : Nat) (i : Fin n) =>
+--      let j := 2*i.1
+--      let hj : j < 2*n := by omega
+--      let j : Fin (2*n) := ⟨j, hj⟩
+--      let k :=
+--        let a := j + j
+--        a + j
+--      j + k)
+--     =
+--     fun (n : Nat) (i : Fin n) =>
+--     let j := 2*i.1
+--     let hj : j < 2*n := by omega
+--     let j : Fin (2*n) := ⟨j, hj⟩
+--     (j + (j + j + j)) := by
+--   (conv => lhs; lsimp)
+
+
+
+
+
+-- set_default_scalar Float
+
+-- open SciLean
+
+-- -- set_option trace.Meta.Tactic.simp.proj true
+-- set_option trace.Meta.Tactic.simp.steps true
+
+
+-- #check (∇ x : Float, let y := x * x; x * y)
+--   rewrite_by
+--     unfold scalarGradient
+--     lsimp
+
+
+-- #check (∂ x : Float, let y := x * x; x * y)
+--   rewrite_by
+--     unfold scalarCDeriv
+--     lsimp
+
+
+-- #check (∂> x : Float, let y := x * x; x * y)
+--   rewrite_by
+--     lsimp
+
+
+-- #check Nat
+
+-- #check (∂> x : Float, let y := x * x; let z := x * y; x * y * z)
+--   rewrite_by
+--     lsimp
+
+set_option profiler true
+
+set_option trace.Meta.Tactic.simp.steps true
+
+set_default_scalar Float
+
+open SciLean
+
+-- #check (∇ x : Float, let y := x * x; let z := x * y; x * y * z)
+--   rewrite_by
+--     unfold scalarGradient
+--     lsimp -- 16107 steps & 4.45s | with cache: 1295 steps && 709ms
+
+
+
+#check (∇ x : Float,
+          let x1 := x * x
+          let x2 := x * x1
+          let x3 := x * x2
+          let x4 := x * x3
+          let x5 := x * x4
+          x * x1 * x2 * x3 * x4 * x5)
+  rewrite_by
+    unfold scalarGradient
+    lsimp -- 16107 steps & 4.45s | with cache: 1295 steps && 709ms
+
+
+
+-- #check (∇ x : Float,
+--           let x1 := x * x
+--           let x2 := x * x1
+--           let x3 := x * x2
+--           let x4 := x * x3
+--           let x5 := x * x4
+--           x * x1 * x2 * x3 * x4 * x5)
+--   rewrite_by
+--     unfold scalarGradient
+--     autodiff
